pset07: finish proving subtype safety

pset07_Subtyping/Pset7.v
@@ -10,208 +10,208 @@ Set Default Goal Selector "!".
 Set Implicit Arguments.
 
 Module Impl.
-(** * Subtyping *)
+  (** * Subtyping *)
 
-(* We can't resist fitting in another crucial aspect of type systems:
- * *subtyping*, which formalizes when any value of one type should also be
- * permitted as a value of some other type. Languages like Java include
- * *nominal* subtyping, based on declared type hierarchies. Instead, here we
- * will prove the soundness of *structural* subtyping, whose rules we'll get to
- * shortly. The simply typed lambda calculus will be our starting point. *)
+  (* We can't resist fitting in another crucial aspect of type systems:
+   * *subtyping*, which formalizes when any value of one type should also be
+   * permitted as a value of some other type. Languages like Java include
+   * *nominal* subtyping, based on declared type hierarchies. Instead, here we
+   * will prove the soundness of *structural* subtyping, whose rules we'll get to
+   * shortly. The simply typed lambda calculus will be our starting point. *)
 
-(* Expression syntax *)
-Inductive exp  :=
-(* Our old friends from simply typed lambda calculus *)
-| Var (x : var)
-| Abs (x : var) (e1 : exp)
-| App (e1 e2 : exp)
+  (* Expression syntax *)
+  Inductive exp  :=
+  (* Our old friends from simply typed lambda calculus *)
+  | Var (x : var)
+  | Abs (x : var) (e1 : exp)
+  | App (e1 e2 : exp)
 
-(* New features, surrounding *tuple* types, which build composite types out of
- * constituents *)
-| TupleNil
-(* Empty tuple (no fields) *)
-| TupleCons (e1 e2 : exp)
-(* Nonempty tuple, where [e1] is the first field of the tuple, and [e2] is a
- * nested tuple with all the remaining fields *)
+  (* New features, surrounding *tuple* types, which build composite types out of
+   * constituents *)
+  | TupleNil
+  (* Empty tuple (no fields) *)
+  | TupleCons (e1 e2 : exp)
+  (* Nonempty tuple, where [e1] is the first field of the tuple, and [e2] is a
+   * nested tuple with all the remaining fields *)
 
-| Proj (e : exp) (n : nat)
-(* Grab the [n]th field of tuple [e]. *)
-.
+  | Proj (e : exp) (n : nat)
+  (* Grab the [n]th field of tuple [e]. *)
+  .
 
-(* Values (final results of evaluation) *)
-Inductive value : exp -> Prop :=
-| VAbs : forall x e1, value (Abs x e1)
-| VTupleNil : value TupleNil
-| VTupleCons : forall e1 e2, value e1 -> value e2 -> value (TupleCons e1 e2)
-.
+  (* Values (final results of evaluation) *)
+  Inductive value : exp -> Prop :=
+  | VAbs : forall x e1, value (Abs x e1)
+  | VTupleNil : value TupleNil
+  | VTupleCons : forall e1 e2, value e1 -> value e2 -> value (TupleCons e1 e2)
+  .
 
-(* The next few definitions are quite routine and should be safe to skim through
- * quickly; but start paying more attention when we get to defining the
- * subtyping relation! *)
+  (* The next few definitions are quite routine and should be safe to skim through
+   * quickly; but start paying more attention when we get to defining the
+   * subtyping relation! *)
 
-(* Substitution (not capture-avoiding, for the usual reason) *)
-Fixpoint subst (e1 : exp) (x : var) (e2 : exp) : exp :=
-  match e2 with
-  | Var y => if y ==v x then e1 else Var y
-  | Abs y e2' => Abs y (if y ==v x then e2' else subst e1 x e2')
-  | App e2' e2'' => App (subst e1 x e2') (subst e1 x e2'')
-  | TupleNil => TupleNil
-  | TupleCons e2' e2'' => TupleCons (subst e1 x e2') (subst e1 x e2'')
-  | Proj e2' n => Proj (subst e1 x e2') n
-  end.
+  (* Substitution (not capture-avoiding, for the usual reason) *)
+  Fixpoint subst (e1 : exp) (x : var) (e2 : exp) : exp :=
+    match e2 with
+    | Var y => if y ==v x then e1 else Var y
+    | Abs y e2' => Abs y (if y ==v x then e2' else subst e1 x e2')
+    | App e2' e2'' => App (subst e1 x e2') (subst e1 x e2'')
+    | TupleNil => TupleNil
+    | TupleCons e2' e2'' => TupleCons (subst e1 x e2') (subst e1 x e2'')
+    | Proj e2' n => Proj (subst e1 x e2') n
+    end.
 
-(* Evaluation contexts *)
-Inductive context :=
-| Hole
-| App1 (C : context) (e2 : exp)
-| App2 (v1 : exp) (C : context)
-| TupleCons1 (C : context) (e2 : exp)
-| TupleCons2 (v1 : exp) (C : context)
-| Proj1 (C : context) (n : nat)
-.
+  (* Evaluation contexts *)
+  Inductive context :=
+  | Hole
+  | App1 (C : context) (e2 : exp)
+  | App2 (v1 : exp) (C : context)
+  | TupleCons1 (C : context) (e2 : exp)
+  | TupleCons2 (v1 : exp) (C : context)
+  | Proj1 (C : context) (n : nat)
+  .
 
-(* Plugging an expression into a context *)
-Inductive plug : context -> exp -> exp -> Prop :=
-| PlugHole : forall e, plug Hole e e
-| PlugApp1 : forall e e' C e2,
-    plug C e e'
-    -> plug (App1 C e2) e (App e' e2)
-| PlugApp2 : forall e e' v1 C,
-    value v1
-    -> plug C e e'
-    -> plug (App2 v1 C) e (App v1 e')
-| PlugTupleCons1 : forall C e e' e2,
-    plug C e e'
-    -> plug (TupleCons1 C e2) e (TupleCons e' e2)
-| PlugTupleCons2 : forall v1 C e e',
-    value v1
-    -> plug C e e'
-    -> plug (TupleCons2 v1 C) e (TupleCons v1 e')
-| PlugProj : forall C e e' n,
-    plug C e e'
-    -> plug (Proj1 C n) e (Proj e' n)
-.
+  (* Plugging an expression into a context *)
+  Inductive plug : context -> exp -> exp -> Prop :=
+  | PlugHole : forall e, plug Hole e e
+  | PlugApp1 : forall e e' C e2,
+      plug C e e'
+      -> plug (App1 C e2) e (App e' e2)
+  | PlugApp2 : forall e e' v1 C,
+      value v1
+      -> plug C e e'
+      -> plug (App2 v1 C) e (App v1 e')
+  | PlugTupleCons1 : forall C e e' e2,
+      plug C e e'
+      -> plug (TupleCons1 C e2) e (TupleCons e' e2)
+  | PlugTupleCons2 : forall v1 C e e',
+      value v1
+      -> plug C e e'
+      -> plug (TupleCons2 v1 C) e (TupleCons v1 e')
+  | PlugProj : forall C e e' n,
+      plug C e e'
+      -> plug (Proj1 C n) e (Proj e' n)
+  .
 
-(* Small-step, call-by-value evaluation *)
-Inductive step0 : exp -> exp -> Prop :=
-| Beta : forall x e v,
-    value v
-    -> step0 (App (Abs x e) v) (subst v x e)
+  (* Small-step, call-by-value evaluation *)
+  Inductive step0 : exp -> exp -> Prop :=
+  | Beta : forall x e v,
+      value v
+      -> step0 (App (Abs x e) v) (subst v x e)
 
-(* To project field 0 out of a tuple, just grab the first component. *)
-| Proj0 : forall v1 v2,
-    value v1
-    -> value v2
-    -> step0 (Proj (TupleCons v1 v2) 0) v1
+  (* To project field 0 out of a tuple, just grab the first component. *)
+  | Proj0 : forall v1 v2,
+      value v1
+      -> value v2
+      -> step0 (Proj (TupleCons v1 v2) 0) v1
 
-(* To project field [1+n], drop the first component and continue with [n]. *)
-| ProjS : forall v1 v2 n,
-    value v1
-    -> value v2
-    -> step0 (Proj (TupleCons v1 v2) (1 + n)) (Proj v2 n)
-.
+  (* To project field [1+n], drop the first component and continue with [n]. *)
+  | ProjS : forall v1 v2 n,
+      value v1
+      -> value v2
+      -> step0 (Proj (TupleCons v1 v2) (1 + n)) (Proj v2 n)
+  .
 
-Inductive step : exp -> exp -> Prop :=
-| StepRule : forall C e1 e2 e1' e2',
-    plug C e1 e1'
-    -> plug C e2 e2'
-    -> step0 e1 e2
-    -> step e1' e2'.
+  Inductive step : exp -> exp -> Prop :=
+  | StepRule : forall C e1 e2 e1' e2',
+      plug C e1 e1'
+      -> plug C e2 e2'
+      -> step0 e1 e2
+      -> step e1' e2'.
 
-Definition trsys_of (e : exp) :=
-  {| Initial := {e}; Step := step |}.
+  Definition trsys_of (e : exp) :=
+    {| Initial := {e}; Step := step |}.
 
-(* Syntax of types *)
-Inductive type :=
-| Fun (dom ran : type)
-| TupleTypeNil
-| TupleTypeCons (t1 t2 : type)
-.
+  (* Syntax of types *)
+  Inductive type :=
+  | Fun (dom ran : type)
+  | TupleTypeNil
+  | TupleTypeCons (t1 t2 : type)
+  .
 
-Inductive subtype : type -> type -> Prop :=
+  Inductive subtype : type -> type -> Prop :=
 
-(* Two function types are related if their components are related pairwise.
- * Counterintuitively, we *reverse* the comparison order for function domains!
- * It may be worth working through some examples to see why the relation would
- * otherwise be unsound. *)
-| StFun : forall t1' t2' t1 t2,
-    subtype t1 t1' ->
-    subtype t2' t2 ->
-    subtype (Fun t1' t2') (Fun t1 t2)
+  (* Two function types are related if their components are related pairwise.
+   * Counterintuitively, we *reverse* the comparison order for function domains!
+   * It may be worth working through some examples to see why the relation would
+   * otherwise be unsound. *)
+  | StFun : forall t1' t2' t1 t2,
+      subtype t1 t1' ->
+      subtype t2' t2 ->
+      subtype (Fun t1' t2') (Fun t1 t2)
 
-(* An empty tuple type is its own subtype. *)
-| StTupleNilNil :
+  (* An empty tuple type is its own subtype. *)
+  | StTupleNilNil :
     subtype TupleTypeNil TupleTypeNil
 
-(* However, a nonempty tuple type is also a subtype of the empty tuple type.
- * This rule gives rise to *width* subtyping, where we can drop some fields of
- * a tuple type to produce a subtype. *)
-| StTupleNilCons : forall t1 t2,
-    subtype (TupleTypeCons t1 t2) TupleTypeNil
+  (* However, a nonempty tuple type is also a subtype of the empty tuple type.
+   * This rule gives rise to *width* subtyping, where we can drop some fields of
+   * a tuple type to produce a subtype. *)
+  | StTupleNilCons : forall t1 t2,
+      subtype (TupleTypeCons t1 t2) TupleTypeNil
 
-(* We also have *depth* subtyping: we can replace tuple components with
- * subtypes. *)
-| StTupleCons : forall t1' t2' t1 t2,
-    subtype t1' t1 ->
-    subtype t2' t2 ->
-    subtype (TupleTypeCons t1' t2') (TupleTypeCons t1 t2)
-.
+  (* We also have *depth* subtyping: we can replace tuple components with
+   * subtypes. *)
+  | StTupleCons : forall t1' t2' t1 t2,
+      subtype t1' t1 ->
+      subtype t2' t2 ->
+      subtype (TupleTypeCons t1' t2') (TupleTypeCons t1 t2)
+  .
 
-(* Here's a more compact notation for subtyping. *)
-Infix "$<:" := subtype (at level 70).
+  (* Here's a more compact notation for subtyping. *)
+  Infix "$<:" := subtype (at level 70).
 
-Local Hint Constructors subtype : core.
+  Local Hint Constructors subtype : core.
 
-(* Projecting out the nth field of a tuple type *)
-Inductive proj_t : type -> nat -> type -> Prop :=
-| ProjT0 : forall t1 t2,
-    proj_t (TupleTypeCons t1 t2) 0 t1
-| ProjTS : forall t1 t2 n t,
-    proj_t t2 n t ->
-    proj_t (TupleTypeCons t1 t2) (1 + n) t
-.
+  (* Projecting out the nth field of a tuple type *)
+  Inductive proj_t : type -> nat -> type -> Prop :=
+  | ProjT0 : forall t1 t2,
+      proj_t (TupleTypeCons t1 t2) 0 t1
+  | ProjTS : forall t1 t2 n t,
+      proj_t t2 n t ->
+      proj_t (TupleTypeCons t1 t2) (1 + n) t
+  .
 
-(* Expression typing relation stating something _has_ a _ty_pe *)
-Inductive has_ty : fmap var type -> exp -> type -> Prop :=
-| HtVar : forall G x t,
-    G $? x = Some t ->
-    has_ty G (Var x) t
-| HtAbs : forall G x e1 t1 t2,
-    has_ty (G $+ (x, t1)) e1 t2 ->
-    has_ty G (Abs x e1) (Fun t1 t2)
-| HtApp : forall G e1 e2 t1 t2,
-    has_ty G e1 (Fun t1 t2) ->
-    has_ty G e2 t1 ->
-    has_ty G (App e1 e2) t2
-| HtTupleNil : forall G,
-    has_ty G TupleNil TupleTypeNil
-| HtTupleCons: forall G e1 e2 t1 t2,
-    has_ty G e1 t1 ->
-    has_ty G e2 t2 ->
-    has_ty G (TupleCons e1 e2) (TupleTypeCons t1 t2)
-| HtProj : forall G e n t t',
-    has_ty G e t' ->
-    proj_t t' n t ->
-    has_ty G (Proj e n) t
+  (* Expression typing relation stating something _has_ a _ty_pe *)
+  Inductive has_ty : fmap var type -> exp -> type -> Prop :=
+  | HtVar : forall G x t,
+      G $? x = Some t ->
+      has_ty G (Var x) t
+  | HtAbs : forall G x e1 t1 t2,
+      has_ty (G $+ (x, t1)) e1 t2 ->
+      has_ty G (Abs x e1) (Fun t1 t2)
+  | HtApp : forall G e1 e2 t1 t2,
+      has_ty G e1 (Fun t1 t2) ->
+      has_ty G e2 t1 ->
+      has_ty G (App e1 e2) t2
+  | HtTupleNil : forall G,
+      has_ty G TupleNil TupleTypeNil
+  | HtTupleCons: forall G e1 e2 t1 t2,
+      has_ty G e1 t1 ->
+      has_ty G e2 t2 ->
+      has_ty G (TupleCons e1 e2) (TupleTypeCons t1 t2)
+  | HtProj : forall G e n t t',
+      has_ty G e t' ->
+      proj_t t' n t ->
+      has_ty G (Proj e n) t
 
-(* This is the crucial rule: when an expression has a type, it also has any
- * supertype of that type. We call this rule *subsumption*. *)
-| HtSub : forall G e t t',
-    has_ty G e t' ->
-    t' $<: t ->
-    has_ty G e t
-.
+  (* This is the crucial rule: when an expression has a type, it also has any
+   * supertype of that type. We call this rule *subsumption*. *)
+  | HtSub : forall G e t t',
+      has_ty G e t' ->
+      t' $<: t ->
+      has_ty G e t
+  .
 
-(* Before we get started proving properties of our type system, please read
- * Pset7Sig.v and consider the questions below. This task is ungraded,
- * but we are assigning it in hopes it helps you complete the
- * following parts.
+  (* Before we get started proving properties of our type system, please read
+   * Pset7Sig.v and consider the questions below. This task is ungraded,
+   * but we are assigning it in hopes it helps you complete the
+   * following parts.
 
- What does it mean for the subtyping order of the arguments in `StFun` to be 
+ What does it mean for the subtyping order of the arguments in `StFun` to be
  reversed?
 
 
- If t1 $<: t2, what is known about some t3 that is a supertype of t2? And 
+ If t1 $<: t2, what is known about some t3 that is a supertype of t2? And
  likewise if it's a subtype of t1?
 
 
@@ -219,13 +219,13 @@ Inductive has_ty : fmap var type -> exp -> type -> Prop :=
  ```
  has_ty G (Abs x e1) t
  ```
- with the `LambdaCalculusAndTypeSoundness` definition of `has_ty`, and what 
+ with the `LambdaCalculusAndTypeSoundness` definition of `has_ty`, and what
  information do you have about `t`?
 
  To contrast, how many goals do you expect with the `has_ty` definition of
- this pset? Why is this the case? 
+ this pset? Why is this the case?
 
- Can you formulate a lemma that consolidates the information present in these 
+ Can you formulate a lemma that consolidates the information present in these
  branches into one conclusion? (Imagine inverting now is equivalent to an
  "or" generating branches for each constructor; can you rephrase a lemma that
  leads to a conclusion with an "and" instead?)
@@ -235,70 +235,309 @@ Inductive has_ty : fmap var type -> exp -> type -> Prop :=
  ```
  has_ty G e (Fun t1 t2)
  ```
- with the `LambdaCalculusAndTypeSoundness` definition of `has_ty`, and what 
- information do you have about `e`? 
+ with the `LambdaCalculusAndTypeSoundness` definition of `has_ty`, and what
+ information do you have about `e`?
 
- To contrast, how many goals do you expect with the `has_ty` definition 
- of this pset? Why is this the case? 
+ To contrast, how many goals do you expect with the `has_ty` definition
+ of this pset? Why is this the case?
 
  Can you formulate a lemma to recover information similar to what inverting
  gave you in FRAP's `has_ty` definition?
 
-*)
+   *)
 
-(* Prove these two basic algebraic properties of subtyping. *)
+  (* Prove these two basic algebraic properties of subtyping. *)
 
-Lemma subtype_refl : forall t1, t1 $<: t1.
-Proof.
-Admitted.
+  Lemma subtype_refl : forall t1, t1 $<: t1.
+  Proof.
+    induct t1; now constructor.
+  Qed.
 
-(* HINT 1 (see Pset7Sig.v) *) 
-Lemma subtype_trans : forall t1 t2 t3, t1 $<: t2 -> t2 $<: t3 -> t1 $<: t3.
-Proof.
-Admitted.
+  Definition subtype_right t1 t2 := forall t3, t2 $<: t3 -> t1 $<: t3.
 
-(* BEGIN handy tactic that we suggest for these proofs *)
-Ltac tac0 :=
-  match goal with
-  | [ H : ex _ |- _ ] => invert H
-  | [ H : _ /\ _ |- _ ] => invert H
-  | [ |- context[_ $+ (?x, _) $? ?y] ] => cases (x ==v y); simplify
-  | [ |- context[?x ==v ?y] ] => cases (x ==v y); simplify
-  | [ H : step _ _ |- _ ] => invert H
-  | [ H : step0 _ _ |- _ ] => invert1 H
-  | [ H : has_ty _ _ _ |- _ ] => invert1 H
-  | [ H : proj_t _ _ _ |- _ ] => invert1 H
-  | [ H : plug _ _ _ |- _ ] => invert1 H
-  | [ H : subtype _ _ |- _ ] => invert1 H
-  | [ H : Some _ = Some _ |- _ ] => invert H
-  end;
-  subst.
+  Definition subtype_left t1 t2 := forall t3, t3 $<: t1 -> t3 $<: t2.
 
-Ltac tac := simplify; subst; propositional; repeat (tac0; simplify); try equality.
-(* END handy tactic *)
+  Lemma subtype_trans_aux t1 t2:
+    t1 $<: t2 -> subtype_left t1 t2 /\ subtype_right t1 t2.
+  Proof.
+    induct 1; split; unfold subtype_left in *; unfold subtype_right in *;
+      intros t3 Ht3; invert Ht3; constructor.
+    - destruct IHsubtype1 as [_ Ht1_right]. apply (Ht1_right t1'0 H4).
+    - destruct IHsubtype2 as [Ht2_left _]. apply (Ht2_left t2'0 H5).
+    - destruct IHsubtype1 as [Ht1_left _]. apply (Ht1_left t0 H3).
+    - destruct IHsubtype2 as [_ Ht2_right]. apply (Ht2_right t4 H5).
+    - destruct IHsubtype1 as [Ht1_left _]. apply (Ht1_left t1'0 H4).
+    - destruct IHsubtype2 as [Ht2_left _]. apply (Ht2_left t2'0 H5).
+    - destruct IHsubtype1 as [_ Ht1_right]. apply (Ht1_right t0 H3).
+    - destruct IHsubtype2 as [_ Ht2_right]. apply (Ht2_right t4 H5).
+  Qed.
+
+  (* HINT 1 (see Pset7Sig.v) *)
+  Lemma subtype_trans : forall t1 t2 t3, t1 $<: t2 -> t2 $<: t3 -> t1 $<: t3.
+  Proof.
+    intros t1 t2 t3 Ht12. pose proof (subtype_trans_aux Ht12) as H.
+    destruct H as [Hleft Hright]. apply Hright.
+  Qed.
+
+  (* BEGIN handy tactic that we suggest for these proofs *)
+  Ltac tac0 :=
+    match goal with
+    | [ H : ex _ |- _ ] => invert H
+    | [ H : _ /\ _ |- _ ] => invert H
+    | [ |- context[_ $+ (?x, _) $? ?y] ] => cases (x ==v y); simplify
+    | [ |- context[?x ==v ?y] ] => cases (x ==v y); simplify
+    | [ H : step _ _ |- _ ] => invert H
+    | [ H : step0 _ _ |- _ ] => invert1 H
+    | [ H : has_ty _ _ _ |- _ ] => invert1 H
+    | [ H : proj_t _ _ _ |- _ ] => invert1 H
+    | [ H : plug _ _ _ |- _ ] => invert1 H
+    | [ H : subtype _ _ |- _ ] => invert1 H
+    | [ H : Some _ = Some _ |- _ ] => invert H
+    end;
+    subst.
+
+  Ltac tac := simplify; subst; propositional; repeat (tac0; simplify); try equality.
+  (* END handy tactic *)
 
 
-(* The real prize: prove soundness of this type system.
- * We suggest starting from a copy of the type-safety proof from the book's
- * EvaluationContexts.v.
- * The soundness argument for simply typed lambda calculus is genuinely difficult
- * (a celebrated result!). We're not expecing you to reinvent it. Rather, the
- * task of this pset is to *extend* it to cover subtyping. This will involve
- * changing some proofs and making appropriate additional helper lemmas (there
- * are more hints in Pset7Sig.v).
- * Trying to write this proof from scratch is *not* recommended for this pset.
- * This is in contrast to the *previous* psets, which we tried to design so that
- * they could be solved from scratch with a good understanding of the lecture
- * material. *)
+  (* The real prize: prove soundness of this type system.
+   * We suggest starting from a copy of the type-safety proof from the book's
+   * EvaluationContexts.v.
+   * The soundness argument for simply typed lambda calculus is genuinely difficult
+   * (a celebrated result!). We're not expecing you to reinvent it. Rather, the
+   * task of this pset is to *extend* it to cover subtyping. This will involve
+   * changing some proofs and making appropriate additional helper lemmas (there
+   * are more hints in Pset7Sig.v).
+   * Trying to write this proof from scratch is *not* recommended for this pset.
+   * This is in contrast to the *previous* psets, which we tried to design so that
+   * they could be solved from scratch with a good understanding of the lecture
+   * material. *)
 
-(* HINT 2-3 (see Pset7Sig.v) *) 
-Theorem safety :
-  forall e t,
-    has_ty $0 e t -> invariantFor (trsys_of e)
-                                  (fun e' => value e'
-                                             \/ exists e'', step e' e'').
-Proof.
-Admitted.
+  (* HINT 2-3 (see Pset7Sig.v) *)
+  Lemma step0_is_step e1 e2:
+    step0 e1 e2 -> step e1 e2.
+  Proof.
+    apply StepRule with (C := Hole) (e1 := e1) (e2 := e2).
+    all: apply PlugHole.
+  Qed.
+
+  Lemma canonical_form_abs e t1 t2 :
+    has_ty $0 e (Fun t1 t2) ->
+    value e ->
+    exists x e1, e = Abs x e1.
+  Proof.
+    (* Use eauto to prove the canonical form, invert Vapp and VProj because they
+     are not values *)
+    induct 1; tac; eauto; invert H1.
+  Qed.
+
+  Lemma canonical_form_tuple e t t1 :
+    has_ty $0 e (TupleTypeCons t t1) ->
+    value e ->
+    exists e1 e2, e = TupleCons e1 e2.
+  Proof.
+    (* Use eauto to prove the canonical form, invert Vapp and VProj because they
+     are not values *)
+    induct 1; tac; eauto; invert H1.
+  Qed.
+
+  Lemma progress : forall e t,
+      has_ty $0 e t
+      -> value e
+        \/ (exists e' : exp, step e e').
+  Proof.
+    induct 1; tac.
+    - left. apply VAbs.           (* Vabs *)
+    - right. apply (canonical_form_abs H) in H3.      (* Vapp *)
+      destruct H3 as [x [e' Habs]]. rewrite Habs. exists (subst e2 x e'). (* step0 *)
+      apply step0_is_step. apply (Beta x e' H1).
+    - right. apply PlugApp1 with (e2 := e2) in H3,H4. exists (App x e2).
+      apply (StepRule H3 H4 H5). (* App e1 e2 where e1 can step *)
+    - right. apply (PlugApp2 H3) in H1,H4. exists (App e1 x).
+      apply (StepRule H1 H4 H5). (* App e1 e2 where e1 is value *)
+    - right. apply PlugApp1 with (e2 := e2) in H3,H6. exists (App x e2).
+      apply (StepRule H3 H6 H7). (* App e1 e2 where both e1 and e2 can step *)
+    - left. apply VTupleNil.
+    - left. apply (VTupleCons H3 H1).
+    - right. apply PlugTupleCons1 with (e2 := e2) in H3,H4. exists (TupleCons x e2).
+      apply (StepRule H3 H4 H5).  (* Cons e1 v2 where e1 can step *)
+    - right. apply (PlugTupleCons2 H3) in H1,H4. exists (TupleCons e1 x).
+      apply (StepRule H1 H4 H5). (* Cons v1 e2 where e2 can step *)
+    - right. apply PlugTupleCons1 with (e2 := e2) in H3,H6. exists (TupleCons x e2).
+      apply (StepRule H3 H6 H7). (* Cons e1 e2 where e1 can step *)
+    - right. invert H0; pose proof (canonical_form_tuple H H1) as Htuple;
+        destruct Htuple as [e1 [e2 Htuple]]; subst e; invert H1;
+        [ exists e1 | exists (Proj e2 n0) ]; (* apply proj0 or projS *)
+        apply step0_is_step; [ apply (Proj0 H3 H4) | apply (ProjS n0 H4 H5) ].
+    - right. apply PlugProj with (n := n) in H1,H3. exists (Proj x n).
+      apply (StepRule H1 H3 H4).  (* Proj e n where e can step *)
+  Qed.
+
+  Lemma weakening_override : forall (G G' : fmap var type) x t,
+      (forall x' t', G $? x' = Some t' -> G' $? x' = Some t')
+      -> (forall x' t', G $+ (x, t) $? x' = Some t'
+                  -> G' $+ (x, t) $? x' = Some t').
+  Proof.
+    simplify.
+    cases (x ==v x'); simplify; eauto.
+  Qed.
+
+  Local Hint Resolve weakening_override : core.
+
+  Lemma weakening : forall G e t,
+      has_ty G e t
+      -> forall G', (forall x t, G $? x = Some t -> G' $? x = Some t)
+              -> has_ty G' e t.
+  Proof.
+    induct 1; tac; try (constructor; eauto).
+    - pose proof (IHhas_ty1 G' H1) as He1. pose proof (IHhas_ty2 G' H1) as He2.
+      apply (HtApp He1 He2).
+    - pose proof (IHhas_ty G' H1) as Hproj. apply (HtProj Hproj H0).
+    - pose proof (IHhas_ty G' H1) as Hsubtype.
+      apply (HtSub Hsubtype H0). (* Subtype *)
+  Qed.
+
+  Local Hint Resolve weakening : core.
+
+  (* Replacing a typing context with an equal one has no effect (useful to guide
+   * proof search as a hint). *)
+  Lemma has_ty_change : forall G e t,
+      has_ty G e t
+      -> forall G', G' = G
+              -> has_ty G' e t.
+  Proof.
+    tac.
+  Qed.
+
+  Local Hint Resolve has_ty_change : core.
+
+  Lemma substitution : forall G x t' e t e',
+      has_ty (G $+ (x, t')) e t
+      -> has_ty $0 e' t'
+      -> has_ty G (subst e' x e) t.
+  Proof.
+    induct 1; tac; try constructor; eauto.
+    - assert (HG: G $+ (x, t') = G $+ (x, t')) by reflexivity.
+      pose proof (IHhas_ty1 G x t'  HG H1) as He1.
+      apply (HtApp He1 H2).
+    - apply (HtProj H2 H0).
+    - apply (HtSub H2 H0).
+  Qed.
+
+  Local Hint Resolve substitution : core.
+
+  Lemma has_ty_abs G x e t1 t2 :
+    has_ty G (Abs x e) (Fun t1 t2) ->
+    exists D S, has_ty (G $+ (x, D)) e S /\ (Fun D S) $<: (Fun t1 t2).
+  Proof.
+    induct 1; tac.
+    - exists t1, t2. split; [ exact H | apply subtype_refl ].
+    - specialize (IHhas_ty x e t1' t2'). specialize ((IHhas_ty eq_refl) eq_refl).
+      destruct IHhas_ty as [D [S [Hty Hsub]]]. exists D, S. split; [ exact Hty | ].
+      apply subtype_trans with (t2 := (Fun t1' t2')); [ exact Hsub | ].
+      apply (StFun H4 H5).
+  Qed.
+
+  Lemma has_ty_app G e1 e2 t:
+    has_ty G (App e1 e2) t ->
+    exists D S, has_ty G e1 (Fun D S) /\ has_ty G e2 D /\ S $<: t.
+  Proof.
+    induct 1; tac.
+    - exists t1, t2. repeat split; auto. apply subtype_refl.
+    - exists x, x0. repeat split; auto. apply (subtype_trans H4 H0).
+  Qed.
+
+  Lemma has_ty_TupleCons G e e' t:
+    has_ty G (TupleCons e e') t ->
+    exists t1 t2, has_ty G e t1 /\ has_ty G e' t2 /\ (TupleTypeCons t1 t2) $<: t.
+  Proof.
+    induct 1; tac.
+    - exists t1, t2. repeat split; eauto. apply subtype_refl.
+    - exists x, x0. repeat split; eauto. apply subtype_trans with (t2 := t'); eauto.
+  Qed.
+
+  Lemma has_ty_proj G e n t:
+    has_ty G (Proj e n) t ->
+    exists t' l, has_ty G e l /\ proj_t l n t' /\ t' $<: t.
+  Proof.
+    induct 1; tac.
+    - exists t, t'. repeat split; eauto. apply subtype_refl.
+    - exists x, x0. repeat split; eauto. apply subtype_trans with (t2 := t'); eauto.
+  Qed.
+
+  Lemma preservation0 : forall e1 e2,
+      step0 e1 e2
+      -> forall t, has_ty $0 e1 t
+             -> has_ty $0 e2 t.
+  Proof.
+    invert 1; tac.
+    - apply has_ty_app in H. destruct H as [t1 [t2 [Habs [Hv Ht1]]]].
+      apply has_ty_abs in Habs. destruct Habs as [ta [tb [Hext Hf]]]. invert Hf.
+      apply substitution with (t' := ta).
+      + apply HtSub with (t' := tb); eauto. apply (subtype_trans H5 Ht1).
+      + apply HtSub with (t' := t1); eauto.
+    - apply has_ty_proj in H. destruct H as [t0 [tl [Hl [Hproj Hsub]]]].
+      apply has_ty_TupleCons in Hl. destruct Hl as [t1 [t2 [Ht1 [Ht2 Hcons]]]].
+      apply HtSub with (t' := t1); [ exact Ht1 | ]. invert Hproj. invert Hcons.
+      apply (subtype_trans H4 Hsub).
+    - apply has_ty_proj in H. destruct H as [t0 [tl [Hl [Hproj Hsub]]]].
+      apply has_ty_TupleCons in Hl. destruct Hl as [t1 [t2 [Ht1 [Ht2 Hcons]]]].
+      invert Hproj. invert Hcons. apply HtSub with (t' := t0); [ | exact Hsub ].
+      apply HtProj with (t' := t4).
+      + apply HtSub with (t' := t2); eauto.
+      + exact H3.
+  Qed.
+
+  Local Hint Resolve preservation0 : core.
+
+  Lemma preservation' : forall C e1 e1',
+      plug C e1 e1'
+      -> forall e2 e2' t, plug C e2 e2'
+                    -> step0 e1 e2
+                    -> has_ty $0 e1' t
+                    -> has_ty $0 e2' t.
+  Proof.
+    induct 1; tac; eauto.
+    - apply has_ty_app in H2. destruct H2 as [t1 [t2 [He' [He2 Hsub]]]].
+      apply HtApp with (t1 := t1); eauto. apply HtSub with (t' := (Fun t1 t2)).
+      + apply IHplug with (e2 := e0); eauto.
+      + constructor; eauto. apply subtype_refl.
+    - apply has_ty_app in H3. destruct H3 as [t1 [t2 [Hv1 [He' Hsub]]]].
+      apply HtApp with (t1 := t1); eauto. (* Use preservation0 for step once *)
+      apply HtSub with (t' := (Fun t1 t2)); eauto. constructor; eauto.
+      apply subtype_refl.
+    - apply has_ty_TupleCons in H2. destruct H2 as [t1 [t2 [He' [He2 Hcons]]]].
+      apply HtSub with (t' := (TupleTypeCons t1 t2)); eauto.
+      apply HtTupleCons; eauto.
+    - apply has_ty_TupleCons in H3. destruct H3 as [t1 [t2 [He' [He2 Hcons]]]].
+      apply HtSub with (t' := (TupleTypeCons t1 t2)); eauto.
+      apply HtTupleCons; eauto.
+    - apply has_ty_proj in H2. destruct H2 as [t' [tl [He' [Hproj Hsub]]]].
+      apply HtSub with (t' := t'); eauto. apply HtProj with (t' := tl); eauto.
+  Qed.
+
+  Local Hint Resolve preservation' : core.
+
+  Lemma preservation : forall e1 e2,
+      step e1 e2
+      -> forall t, has_ty $0 e1 t
+             -> has_ty $0 e2 t.
+  Proof.
+    invert 1; tac; eauto.
+  Qed.
+
+  Local Hint Resolve progress preservation : core.
+
+  Theorem safety :
+    forall e t,
+      has_ty $0 e t -> invariantFor (trsys_of e)
+                        (fun e' => value e'
+                                \/ exists e'', step e' e'').
+  Proof.
+    simplify.
+    apply invariant_weaken with (invariant1 := fun e' => has_ty $0 e' t); eauto.
+    apply invariant_induction; simplify; eauto; equality.
+  Qed.
 
 End Impl.
 
